Remove liftType from user-interface of iter

iodiv/DivFreeTauDM.fst
@@ -19,11 +19,30 @@ open DivFreeTauSpec
 type action_iwp (sg : signature) =
   ac : sg.act -> x : sg.arg ac -> iwp (sg.res x)
 
+let i_unLift #a (w : iwp (liftType u#a a)) : iwp a =
+  i_bind w (fun x -> i_ret (unLift x))
+
+// i_iter but with the liftType
+let i_iter_lift (#index : Type0) (#a : Type0) (w : index -> iwp (liftType u#a (either index a))) (i : index) : iwp a =
+  i_iter (fun j -> i_unLift (w j)) i
+
+let i_iter_lift_mono (#index : Type0) (#a : Type0) (w w' : index -> iwp (liftType u#a (either index a))) (i : index) :
+  Lemma
+    (requires forall j. w j `ile` w' j)
+    (ensures i_iter_lift w i `ile` i_iter_lift w' i)
+= ()
+
+let i_iter_lift_cong (#index : Type0) (#a : Type0) (w w' : index -> iwp (liftType u#a (either index a))) (i : index) :
+  Lemma
+    (requires forall j. w j `ieq` w' j)
+    (ensures i_iter_lift w i `ieq` i_iter_lift w' i)
+= i_iter_lift_mono w w' i ; i_iter_lift_mono w' w i
+
 let rec theta (#a : Type u#a) #sg (w_act : action_iwp sg) (c : m sg a) : iwp a =
   match c with
   | Ret x -> i_ret x
   | Req pre k -> i_bind (i_req pre) (fun x -> theta w_act (k x))
-  | Iter index b f i k -> i_bind (i_iter u#a (fun j -> theta w_act (f j)) i) (fun x -> theta w_act (k x))
+  | Iter index b f i k -> i_bind (i_iter_lift u#a (fun j -> theta w_act (f j)) i) (fun x -> theta w_act (k x))
   | Call ac x k -> i_bind (w_act ac x) (fun x -> theta w_act (k x))
 
 let theta_ret #a #sg (w_act : action_iwp sg) (x : a) :
@@ -61,22 +80,22 @@ let rec theta_reType #sg (#d : Type0) (w_act : action_iwp sg) (c : m u#a sg (lif
     end ;
 
     calc (ieq) {
-      i_iter (fun j -> theta w_act (m_reType (g j))) i ;
-      `ieq` { i_iter_cong (fun j -> theta w_act (m_reType (g j))) (fun j -> theta w_act (g j)) i }
-      i_iter (fun j -> theta w_act (g j)) i ;
+      i_iter_lift (fun j -> theta w_act (m_reType (g j))) i ;
+      `ieq` { i_iter_lift_cong (fun j -> theta w_act (m_reType (g j))) (fun j -> theta w_act (g j)) i }
+      i_iter_lift (fun j -> theta w_act (g j)) i ;
     } ;
-    assert (i_iter (fun j -> theta w_act (g j)) i `ieq` i_iter (fun j -> theta w_act (m_reType (g j))) i) ;
+    assert (i_iter_lift (fun j -> theta w_act (g j)) i `ieq` i_iter_lift (fun j -> theta w_act (m_reType (g j))) i) ;
 
     calc (ieq) {
       theta w_act c ;
       == {}
       theta w_act (Iter index ct g i k) ;
       == { _ by (compute ()) }
-      i_bind (i_iter (fun j -> theta w_act (g j)) i) (fun x -> theta w_act (k x)) ;
-      `ieq` { i_bind_cong (i_iter (fun j -> theta w_act (g j)) i) (fun x -> theta w_act (k x)) (fun x -> theta w_act (m_reType (k x))) }
-      i_bind (i_iter (fun j -> theta w_act (g j)) i) (fun x -> theta w_act (m_reType (k x))) ;
+      i_bind (i_iter_lift (fun j -> theta w_act (g j)) i) (fun x -> theta w_act (k x)) ;
+      `ieq` { i_bind_cong (i_iter_lift (fun j -> theta w_act (g j)) i) (fun x -> theta w_act (k x)) (fun x -> theta w_act (m_reType (k x))) }
+      i_bind (i_iter_lift (fun j -> theta w_act (g j)) i) (fun x -> theta w_act (m_reType (k x))) ;
       `ieq` {}
-      i_bind (i_iter (fun j -> theta w_act (m_reType (g j))) i) (fun x -> theta w_act (m_reType (k x))) ;
+      i_bind (i_iter_lift (fun j -> theta w_act (m_reType (g j))) i) (fun x -> theta w_act (m_reType (k x))) ;
       == { _ by (compute ()) }
       theta w_act (Iter index ct (fun j -> m_reType (g j)) i (fun y -> m_reType (k y))) ;
       == {}
@@ -160,9 +179,9 @@ let rec theta_bind (#a : Type u#a) (#b : Type u#b) #sg (w_act : action_iwp sg) (
     assert (forall j. theta w_act (g j) `ile` theta w_act (m_reType (g j))) ;
 
     calc (ile) {
-      i_iter (fun j -> theta w_act (m_reType (g j))) i ;
-      `ile` { i_iter_mono (fun j -> theta w_act (m_reType (g j))) (fun j -> theta w_act (g j)) i }
-      i_iter (fun j -> theta w_act (g j)) i ;
+      i_iter_lift (fun j -> theta w_act (m_reType (g j))) i ;
+      `ile` { i_iter_lift_mono (fun j -> theta w_act (m_reType (g j))) (fun j -> theta w_act (g j)) i }
+      i_iter_lift (fun j -> theta w_act (g j)) i ;
     } ;
 
     calc (ile) {
@@ -172,13 +191,13 @@ let rec theta_bind (#a : Type u#a) (#b : Type u#b) #sg (w_act : action_iwp sg) (
       == { _ by (compute ()) }
       theta w_act (Iter index ct (fun j -> m_reType (g j)) i (fun y -> m_bind (k y) f)) ;
       == { _ by (compute ()) }
-      i_bind (i_iter (fun j -> theta w_act (m_reType (g j))) i) (fun x -> theta w_act (m_bind (k x) f)) ;
+      i_bind (i_iter_lift (fun j -> theta w_act (m_reType (g j))) i) (fun x -> theta w_act (m_bind (k x) f)) ;
       `ile` {} // If need be, can use w_bind_mono explicitly
-      i_bind (i_iter (fun j -> theta w_act (g j)) i) (fun x -> theta w_act (m_bind (k x) f)) ;
-      `ile` { i_bind_mono (i_iter (fun j -> theta w_act (g j)) i) (fun x -> theta w_act (m_bind (k x) f)) (fun x -> i_bind (theta w_act (k x)) (fun x -> theta w_act (f x))) }
-      i_bind (i_iter (fun j -> theta w_act (g j)) i) (fun x -> i_bind (theta w_act (k x)) (fun x -> theta w_act (f x))) ;
-      `ile` { i_bind_assoc (i_iter (fun j -> theta w_act (g j)) i) (fun x -> theta w_act (k x)) (fun x -> theta w_act (f x)) }
-      i_bind (i_bind (i_iter (fun j -> theta w_act (g j)) i) (fun x -> theta w_act (k x))) (fun x -> theta w_act (f x)) ;
+      i_bind (i_iter_lift (fun j -> theta w_act (g j)) i) (fun x -> theta w_act (m_bind (k x) f)) ;
+      `ile` { i_bind_mono (i_iter_lift (fun j -> theta w_act (g j)) i) (fun x -> theta w_act (m_bind (k x) f)) (fun x -> i_bind (theta w_act (k x)) (fun x -> theta w_act (f x))) }
+      i_bind (i_iter_lift (fun j -> theta w_act (g j)) i) (fun x -> i_bind (theta w_act (k x)) (fun x -> theta w_act (f x))) ;
+      `ile` { i_bind_assoc (i_iter_lift (fun j -> theta w_act (g j)) i) (fun x -> theta w_act (k x)) (fun x -> theta w_act (f x)) }
+      i_bind (i_bind (i_iter_lift (fun j -> theta w_act (g j)) i) (fun x -> theta w_act (k x))) (fun x -> theta w_act (f x)) ;
       == { _ by (compute ()) }
       i_bind (theta w_act (Iter index ct g i k)) (fun x -> theta w_act (f x)) ;
       == {}
@@ -214,6 +233,78 @@ let rec theta_bind (#a : Type u#a) (#b : Type u#b) #sg (w_act : action_iwp sg) (
     i_bind_mono (w_act ac x) (fun x -> theta w_act (m_bind (k x) f)) (fun x -> i_bind (theta w_act (k x)) (fun x -> theta w_act (f x))) ;
 
     ile_trans (theta w_act (m_bind c f)) (i_bind (w_act ac x) (fun x -> i_bind (theta w_act (k x)) (fun x -> theta w_act (f x)))) (i_bind (theta w_act c) (fun x -> theta w_act (f x)))
+
+let rec theta_map_as_bind #sg (w_act : action_iwp sg) (#a : Type u#a) (#b : Type u#b) (f : a -> b) (c : m sg a) :
+  Lemma (theta w_act (m_map f c) `ieq` theta w_act (m_bind c (fun x -> m_ret (f x))))
+= match c with
+  | Ret x -> ()
+
+  | Req pre k ->
+
+    introduce forall x. theta w_act (m_map f (k x)) `ieq` theta w_act (m_bind (k x) (fun x -> m_ret (f x)))
+    with begin
+      theta_map_as_bind w_act f (k x)
+    end
+
+  | Iter index d g i k ->
+
+    assert_norm (m_map f (Iter index d g i k) == Iter index d (fun j -> m_map reType (g j)) i (fun y -> m_map f (k y))) ;
+    assert_norm (m_bind (Iter index d g i k) (fun x -> m_ret (f x)) == Iter index d (fun j -> m_map reType (g j)) i (fun y -> m_bind (k y) (fun x -> m_ret (f x)))) ;
+
+    introduce forall x. theta w_act (m_map f (k x)) `ieq` theta w_act (m_bind (k x) (fun x -> m_ret (f x)))
+    with begin
+      theta_map_as_bind w_act f (k x)
+    end ;
+
+    calc (ieq) {
+      theta w_act (m_map f c) ;
+      == {}
+      theta w_act (Iter index d (fun j -> m_map reType (g j)) i (fun y -> m_map f (k y))) ;
+      == { _ by (compute ()) }
+      i_bind (i_iter_lift (fun j -> theta w_act (m_map reType (g j))) i) (fun x -> theta w_act (m_map f (k x))) ;
+      `ieq` { i_bind_cong (i_iter_lift (fun j -> theta w_act (m_map reType (g j))) i) (fun x -> theta w_act (m_map f (k x))) (fun x -> theta w_act (m_bind (k x) (fun x -> m_ret (f x)))) }
+      i_bind (i_iter_lift (fun j -> theta w_act (m_map reType (g j))) i) (fun x -> theta w_act (m_bind (k x) (fun x -> m_ret (f x)))) ;
+      == { _ by (compute ()) }
+      theta w_act (Iter index d (fun j -> m_map reType (g j)) i (fun y -> m_bind (k y) (fun x -> m_ret (f x)))) ;
+      == {}
+      theta w_act (m_bind c (fun x -> m_ret (f x))) ;
+    }
+
+  | Call ac x k ->
+
+    assert_norm (m_map f (Call ac x k) == Call ac x (fun y -> m_map f (k y))) ;
+    assert_norm (m_bind (Call ac x k) (fun x -> m_ret (f x)) == Call ac x (fun y -> m_bind (k y) (fun x -> m_ret (f x)))) ;
+
+    introduce forall x. theta w_act (m_map f (k x)) `ieq` theta w_act (m_bind (k x) (fun x -> m_ret (f x)))
+    with begin
+      theta_map_as_bind w_act f (k x)
+    end ;
+
+    calc (ieq) {
+      theta w_act (m_map f c) ;
+      == {}
+      theta w_act (Call ac x (fun y -> m_map f (k y))) ;
+      == { _ by (compute ()) }
+      i_bind (w_act ac x) (fun x -> theta w_act (m_map f (k x))) ;
+      `ieq` { i_bind_cong (w_act ac x) (fun x -> theta w_act (m_map f (k x))) (fun x -> theta w_act (m_bind (k x) (fun x -> m_ret (f x)))) }
+      i_bind (w_act ac x) (fun x -> theta w_act (m_bind (k x) (fun x -> m_ret (f x)))) ;
+      == { _ by (compute ()) }
+      theta w_act (Call ac x (fun y -> m_bind (k y) (fun x -> m_ret (f x)))) ;
+      == {}
+      theta w_act (m_bind c (fun x -> m_ret (f x))) ;
+    }
+
+let theta_map (#a : Type u#a) (#b : Type u#b) #sg (w_act : action_iwp sg) (f : a -> b) (c : m sg a) :
+  Lemma (theta w_act (m_map f c) `ile` i_bind (theta w_act c) (fun x -> i_ret (f x)))
+= calc (ile) {
+    theta w_act (m_map f c) ;
+    `ieq` { theta_map_as_bind w_act f c }
+    theta w_act (m_bind c (fun x -> m_ret (f x))) ;
+    `ile` { theta_bind w_act c (fun x -> m_ret (f x)) }
+    i_bind (theta w_act c) (fun x -> theta w_act (m_ret (f x))) ;
+    `ile` { i_bind_mono (theta w_act c) (fun x -> theta w_act (m_ret (f x))) (fun x -> i_ret (f x)) }
+    i_bind (theta w_act c) (fun x -> i_ret (f x)) ;
+  }
 
 let theta_req #a #sg (w_act : action_iwp sg) (pre : pure_pre) :
   Lemma (theta w_act (m_req pre) `ile` i_req pre)
@@ -261,16 +352,53 @@ let dm_call #sg (#w_act : action_iwp sg) (ac : sg.act) (x : sg.arg ac) : dm sg w
   } ;
   m_call ac x
 
-let dm_iter #sg #w_act #index #b #w (f : (j : index) -> dm sg w_act (liftType (either index b)) (w j)) (i : index) : dm sg w_act b (i_iter w i) =
+let i_unlift_lift #a (w : iwp a) :
+  Lemma (i_unLift (i_bind w (fun x -> i_ret (LiftTy x))) `ile` w)
+= introduce forall post hist. w post hist ==> i_unLift (i_bind w (fun x -> i_ret (LiftTy x))) post hist
+  with begin
+    calc (==) {
+      i_unLift (i_bind w (fun x -> i_ret (LiftTy x))) post hist ;
+      == {}
+      i_bind (i_bind w (fun x -> i_ret (LiftTy x))) (fun x -> i_ret (unLift x)) post hist ;
+      == {}
+      i_bind w (fun x -> i_ret (LiftTy x)) (i_bind_post (fun x -> i_ret (unLift x)) post hist) hist ;
+      == {}
+      w (i_bind_post (fun x -> i_ret (LiftTy x)) (i_bind_post (fun x -> i_ret (unLift x)) post hist) hist) hist ;
+    } ;
+    introduce forall r. post r ==> i_bind_post (fun x -> i_ret (LiftTy x)) (i_bind_post (fun x -> i_ret (unLift x)) post hist) hist r
+    with begin
+      match r with
+      | Ocv tr x -> ()
+      | Odv s -> ()
+    end ;
+    assert (post `i_post_le` i_bind_post (fun x -> i_ret (LiftTy x)) (i_bind_post (fun x -> i_ret (unLift x)) post hist) hist)
+  end
+
+let dm_iter #sg #w_act #index #b #w (f : (j : index) -> dm sg w_act (either index b) (w j)) (i : index) : dm sg w_act b (i_iter w i) =
+
+  introduce forall j. theta w_act (m_map LiftTy (f j)) `ile` i_bind (theta w_act (f j)) (fun x -> i_ret (LiftTy x))
+  with begin
+    theta_map w_act LiftTy (f j)
+  end ;
+
+  introduce forall j. i_unLift (i_bind (theta w_act (f j)) (fun x -> i_ret (LiftTy x))) `ile` w j
+  with begin
+    i_unlift_lift (theta w_act (f j))
+  end ;
+
   calc (ile) {
     theta w_act (m_iter f i) ;
     == { _ by (compute ()) }
-    i_bind (i_iter (fun j -> theta w_act (f j)) i) (fun x -> theta w_act (m_ret x)) ;
-    `ile` { i_bind_mono (i_iter (fun j -> theta w_act (f j)) i) (fun x -> theta w_act (m_ret x)) i_ret }
-    i_bind (i_iter (fun j -> theta w_act (f j)) i) i_ret ;
-    `ile` { i_bind_ret (i_iter (fun j -> theta w_act (f j)) i) }
-    i_iter (fun j -> theta w_act (f j)) i ;
-    `ile` {}
+    i_bind (i_iter_lift (fun j -> theta w_act (m_map LiftTy (f j))) i) (fun x -> theta w_act (m_ret x)) ;
+    `ile` { i_bind_mono (i_iter_lift (fun j -> theta w_act (m_map LiftTy (f j))) i) (fun x -> theta w_act (m_ret x)) i_ret }
+    i_bind (i_iter_lift (fun j -> theta w_act (m_map LiftTy (f j))) i) i_ret ;
+    `ile` { i_bind_ret (i_iter_lift (fun j -> theta w_act (m_map LiftTy (f j))) i) }
+    i_iter_lift (fun j -> theta w_act (m_map LiftTy (f j))) i ;
+    `ile` { i_iter_lift_mono (fun j -> theta w_act (m_map LiftTy (f j))) (fun j -> i_bind (theta w_act (f j)) (fun x -> i_ret (LiftTy x))) i }
+    i_iter_lift (fun j -> i_bind (theta w_act (f j)) (fun x -> i_ret (LiftTy x))) i ;
+    == { _ by (compute ()) }
+    i_iter (fun j -> i_unLift (i_bind (theta w_act (f j)) (fun x -> i_ret (LiftTy x)))) i ;
+    `ile` { i_iter_mono (fun j -> i_unLift (i_bind (theta w_act (f j)) (fun x -> i_ret (LiftTy x)))) w i }
     i_iter w i ;
   } ;
   m_iter f i
