iodiv/DivFree.fst
@@ -24,18 +24,18 @@ let m_ret #sg #a (x : a) : m sg a =
 let m_req #sg (pre : pure_pre) : m sg (squash pre) =
   Req pre (fun h -> m_ret h)
 
-let m_iter #sg #index #b (f : index -> m sg (liftType (either index b))) (i : index) : m sg b =
-  Iter index b f i (fun x -> m_ret x)
-
-let m_call #sg (ac : sg.act) (x : sg.arg ac) : m sg (sg.res x) =
-  Call ac x (fun y -> m_ret y)
-
 let rec m_map #sg (#a : Type u#a) (#b : Type u#b) (f : a -> b) (c : m sg a) : m sg b =
   match c with
   | Ret x -> Ret (f x)
   | Req pre k -> Req pre (fun h -> m_map f (k h))
   | Iter index d g i k -> Iter index d (fun j -> m_map reType (g j)) i (fun y -> m_map f (k y))
   | Call ac x k -> Call ac x (fun y -> m_map f (k y))
+
+let m_iter #sg #index #b (f : index -> m sg (either index b)) (i : index) : m sg b =
+  Iter index b (fun j -> m_map LiftTy (f j)) i (fun x -> m_ret x)
+
+let m_call #sg (ac : sg.act) (x : sg.arg ac) : m sg (sg.res x) =
+  Call ac x (fun y -> m_ret y)
 
 // Could also define m_reType without going through m_map
 let m_reType #sg (#d : Type0) (c : m u#a sg (liftType d)) : m u#b sg (liftType d) =
